src/spec/TLS13.ConnectionState.ProtectedWireLemmas.fsti
@@ -1987,6 +1987,123 @@ val lemma_protected_handshake_event_projection_pair_after_server_write_client_re
             client_tail_received
             client_final)
 
+val lemma_protected_handshake_event_projection_pair_after_client_write_server_read_install_heads_with_tails
+  (client:CS.connection_model)
+  (server:CS.connection_model)
+  (client_material:CS.traffic_key_material)
+  (server_material:CS.traffic_key_material)
+  (sent_msg:M.handshake_msg)
+  (received_msg:M.handshake_msg)
+  (client_rest:list CS.conn_event)
+  (server_rest:list CS.conn_event)
+  (client_raw_sent:B.bytes)
+  (client_raw_received:B.bytes)
+  (server_raw_sent:B.bytes)
+  (server_raw_received:B.bytes)
+  (client_final:CS.connection_model)
+  (server_final:CS.connection_model)
+  : Lemma
+      (requires
+        (match
+          client.CS.model_handshake.CS.hs_keys.CS.ks_handshake_secret,
+          server.CS.model_handshake.CS.hs_keys.CS.ks_handshake_secret
+        with
+        | Some client_secret, Some server_secret ->
+          Seq.equal client_secret server_secret
+        | _, _ ->
+          False) /\
+        Seq.equal
+          client.CS.model_handshake.CS.hs_transcript
+          server.CS.model_handshake.CS.hs_transcript /\
+        Seq.equal client_raw_sent server_raw_received /\
+        protected_handshake_wire_round_trip_message sent_msg /\
+        protected_handshake_wire_round_trip_message received_msg /\
+        CS.conn_events_sent_seal_replay
+          client
+          (CS.ConnLocalEvent
+            (CS.LocalInstallTrafficKeys {
+              CS.install_epoch = CS.TrafficHandshake;
+              CS.install_direction = CS.TrafficWrite;
+              CS.install_material = client_material;
+            }) :: CS.ConnNetworkEvent {
+              CL.message_direction = CL.Sent;
+              CL.message_value = M.TlsHandshake sent_msg;
+            } :: client_rest)
+          client_raw_sent
+          client_raw_received
+          client_final /\
+        CS.conn_events_received_decode_replay
+          server
+          (CS.ConnLocalEvent
+            (CS.LocalInstallTrafficKeysForRole {
+              CS.install_role = CS.ServerEndpoint;
+              CS.install_payload = {
+                CS.install_epoch = CS.TrafficHandshake;
+                CS.install_direction = CS.TrafficRead;
+                CS.install_material = server_material;
+              };
+            }) :: CS.ConnNetworkEvent {
+              CL.message_direction = CL.Received;
+              CL.message_value = M.TlsHandshake received_msg;
+            } :: server_rest)
+          server_raw_sent
+          server_raw_received
+          server_final)
+      (ensures
+        exists client_after server_after client_after_head server_after_head pair
+          client_tail_sent client_tail_received
+          server_tail_sent server_tail_received.
+          CS.step_model
+            client
+            (CS.ConnLocalEvent
+              (CS.LocalInstallTrafficKeys {
+                CS.install_epoch = CS.TrafficHandshake;
+                CS.install_direction = CS.TrafficWrite;
+                CS.install_material = client_material;
+              })) == Some client_after /\
+          CS.step_model
+            server
+            (CS.ConnLocalEvent
+              (CS.LocalInstallTrafficKeysForRole {
+                CS.install_role = CS.ServerEndpoint;
+                CS.install_payload = {
+                  CS.install_epoch = CS.TrafficHandshake;
+                  CS.install_direction = CS.TrafficRead;
+                  CS.install_material = server_material;
+                };
+              })) == Some server_after /\
+          CS.step_model
+            client_after
+            (CS.ConnNetworkEvent {
+              CL.message_direction = CL.Sent;
+              CL.message_value = M.TlsHandshake sent_msg;
+            }) == Some client_after_head /\
+          CS.step_model
+            server_after
+            (CS.ConnNetworkEvent {
+              CL.message_direction = CL.Received;
+              CL.message_value = M.TlsHandshake received_msg;
+            }) == Some server_after_head /\
+          pair.pm_sender == client_after /\
+          pair.pm_receiver == server_after /\
+          protected_handshake_event_projection_pair
+            pair
+            sent_msg
+            received_msg /\
+          Seq.equal client_tail_sent server_tail_received /\
+          CS.conn_events_sent_seal_replay
+            client_after_head
+            client_rest
+            client_tail_sent
+            client_tail_received
+            client_final /\
+          CS.conn_events_received_decode_replay
+            server_after_head
+            server_rest
+            server_tail_sent
+            server_tail_received
+            server_final)
+
 val lemma_protected_handshake_event_projection_pair_after_sender_received_network_head
   (sender:CS.connection_model)
   (receiver:CS.connection_model)
